linking/linking.v
@@ -17,6 +17,8 @@ Require Import Integers.
 
 Require Import ZArith.
 
+Require Import gen_genv.
+
 (* This file is a parametric version of [compcert_linking.v].  See that   *)
 (* file for more information.                                             *)
 
@@ -30,12 +32,13 @@ Require Import ZArith.
 
 Module Modsem. 
 
-Record t (M : Type) := mk
-  { F   : Type
-  ; V   : Type
-  ; ge  : Genv.t F V
+(* V is the value type used to communicate with the outside world. *)
+Record t (M : Type) (V : Type) (T : Type) := mk
+  { G   : Type
+  ; global : @GlobalEnv G V
+  ; ge  : G
   ; C   : Type
-  ; sem : @CoreSemantics (Genv.t F V) C M }.
+  ; sem : @CoreSemantics G C M V T }.
 
 End Modsem.
 
@@ -43,16 +46,16 @@ End Modsem.
 
 Module Core. Section core.
 
-Variable M : Type.
+Variables M V T : Type.
 Variable N : pos.
-Variable cores : 'I_N -> Modsem.t M.
+Variable cores : 'I_N -> Modsem.t M V T.
 
 Import Modsem.
 
 Record t := mk
   { i  : 'I_N
   ; c  :> (cores i).(C) 
-  ; sg : signature }.
+  ; sg : g_signature T }.
 
 Definition upd (core : t) (newC : (cores core.(i)).(C)) :=
   {| i := core.(i)
@@ -61,15 +64,15 @@ Definition upd (core : t) (newC : (cores core.(i)).(C)) :=
 
 End core. End Core.
 
-Arguments Core.t {M N} cores.
+Arguments Core.t {M V T N} cores.
 
-Arguments Core.i {M N cores} !t /.
+Arguments Core.i {M V T N cores} !t /.
 
-Arguments Core.c {M N cores} !t /.
+Arguments Core.c {M V T N cores} !t /.
 
-Arguments Core.sg {M N cores} !t /.
+Arguments Core.sg {M V T N cores} !t /.
 
-Arguments Core.upd {M N cores} !core _ /.
+Arguments Core.upd {M V T N cores} !core _ /.
 
 (* Linking semantics invariants:                                          *)
 (*  -All cores except the topmost one are at_external.                    *)
@@ -79,17 +82,16 @@ Section coreDefs.
 
 Import Modsem.
 
-Variable M : Type.
+Variables M V T : Type.
 Variable N : pos.
-Variable cores : 'I_N -> Modsem.t M.
+Variable cores : 'I_N -> Modsem.t M V T.
 
 Definition atExternal (c: Core.t cores) :=
   let: (Core.mk i c sg) := c in
-  let: F := (cores i).(F) in
-  let: V := (cores i).(V) in
+  let: G := G (cores i) in
   let: C := (cores i).(C) in
   let: sem := (cores i).(sem) in
-  if @at_external (Genv.t F V) C M sem c is 
+  if @at_external G C M V T sem c is 
     Some (ef, dep_sig, args) then true
   else false.
 
@@ -98,13 +100,13 @@ Definition wf_callStack (stk : Stack.t (Core.t cores)) :=
 
 End coreDefs.
 
-Arguments atExternal {M N} cores c.
+Arguments atExternal {M V T N} cores c.
 
 (** Call stacks are [stack]s satisfying the [wf_callStack] invariant. *)
 
 Module CallStack. Section callStack.
 
-Context {M : Type} {N : pos} (cores : 'I_N -> Modsem.t M).
+Context {M V T : Type} {N : pos} (cores : 'I_N -> Modsem.t M V T).
 
 Record t : Type := mk
   { callStack :> Stack.t (Core.t cores)
@@ -149,9 +151,9 @@ End callStack. End CallStack.
 
 Module Linker. Section linker.
 
-Variable M : Type.
+Variables M V T : Type.
 Variable N : pos.
-Variable cores : 'I_N  -> Modsem.t M.
+Variable cores : 'I_N  -> Modsem.t M V T.
 
 Record t := mkLinker 
   { fn_tbl : ident -> option 'I_N
@@ -165,7 +167,7 @@ Notation linker := Linker.t.
 
 Section linkerDefs.
 
-Context {M : Type} {N : pos} (my_cores : 'I_N -> Modsem.t M) (l : linker N my_cores).
+Context {M V T : Type} {N : pos} (my_cores : 'I_N -> Modsem.t M V T) (l : linker N my_cores).
 
 Import CallStack. (*for coercion [callStack]*)
 
@@ -236,9 +238,9 @@ Definition emptyStack := if l.(stack).(callStack) is [::] then true else false.
 
 Import Modsem.
 
-Definition initCore (sg: signature) (ix: 'I_N) (v: val) (args: list val) 
+Definition initCore (sg: g_signature T) (ix: 'I_N) (v: V) (args: list V)
   : option (Core.t my_cores):=
-  if @initial_core _ _ _ 
+  if @initial_core _ _ _ _ _
        (my_cores ix).(sem)
        (my_cores ix).(Modsem.ge) 
        v args 
@@ -247,22 +249,20 @@ Definition initCore (sg: signature) (ix: 'I_N) (v: val) (args: list val)
 
 End linkerDefs.
 
-Notation ge_ty := (Genv.t unit unit).
+Arguments updStack {M V T N} {my_cores} !_ _ /.
 
-Arguments updStack {M N} {my_cores} !_ _ /.
+Arguments updCore {M V T N} {my_cores} !_ _ /.
 
-Arguments updCore {M N} {my_cores} !_ _ /.
+Arguments pushCore {M V T N} {my_cores} !l _ _ /.
 
-Arguments pushCore {M N} {my_cores} !l _ _ /.
+Arguments peekCore {M V T N} {my_cores} !l /.
 
-Arguments peekCore {M N} {my_cores} !l /.
+Arguments emptyStack {M V T N} {my_cores} !l /.
 
-Arguments emptyStack {M N} {my_cores} !l /.
-
-Lemma popCoreI M N my_cores l l' pf : 
+Lemma popCoreI M V T N my_cores l l' pf : 
   inContext l -> 
   l' = updStack l (CallStack.mk (STACK.pop (CallStack.callStack l)) pf) ->
-  @popCore M N my_cores l = Some l'.
+  @popCore M V T N my_cores l = Some l'.
 Proof.
 rewrite /popCore.
 move: (popCore_obligation_1 l); move: (popCore_obligation_2 l).
@@ -273,8 +273,8 @@ f_equal=> //.
 by apply: proof_irr.
 Qed.
 
-Lemma popCoreE M N my_cores l l' : 
-  @popCore M N my_cores l = Some l' ->
+Lemma popCoreE M V T N my_cores l l' : 
+  @popCore M V T N my_cores l = Some l' ->
   exists pf,
   [/\ inContext l
     & l' = updStack l (CallStack.mk (STACK.pop (CallStack.callStack l)) pf)].
@@ -295,8 +295,10 @@ Qed.
 Module LinkerSem. Section linkerSem.
 
 Variable M : Type.
+Context `(global : GlobalEnv).
+Variable T : Type.
 Variable N : pos.  (* Number of (compile-time) modules *)
-Variable my_cores : 'I_N  -> Modsem.t M.
+Variable my_cores : 'I_N  -> Modsem.t M V T.
 Variable my_fn_tbl: ident -> option 'I_N.
 
 (* [handle id l args] looks up function id [id] in function table         *)
@@ -306,7 +308,7 @@ Variable my_fn_tbl: ident -> option 'I_N.
 
 Section handle.
 
-Variables (sg: signature) (id: ident) (l: linker N my_cores) (args: list val).
+Variables (sg: g_signature T) (id: ident) (l: linker N my_cores) (args: list V).
 
 Import CallStack.
 
@@ -316,8 +318,8 @@ Definition handle :=
                -> option (linker N my_cores)) with
     | true => fun pf => 
         if l.(fn_tbl) id is Some ix then
-        if Genv.find_symbol (my_cores ix).(Modsem.ge) id is Some bf then
-        if initCore my_cores sg ix (Vptr bf Int.zero) args is Some c 
+        if @find_symbol _ _ (my_cores ix).(Modsem.global) (my_cores ix).(Modsem.ge) id is Some v then
+        if initCore my_cores sg ix v args is Some c 
           then Some (pushCore l c (Logic.eq_sym pf))
         else None else None else None
     | false => fun _ => None
@@ -331,10 +333,10 @@ Import CallStack.
 
 Lemma handleP sg id l args l' :
   handle sg id l args = Some l' <-> 
-  (exists (pf : all (atExternal my_cores) l.(stack).(callStack)) ix bf c,
+  (exists (pf : all (atExternal my_cores) l.(stack).(callStack)) ix v c,
      [/\ l.(fn_tbl) id = Some ix 
-       , Genv.find_symbol (my_cores ix).(Modsem.ge) id = Some bf
-       , initCore my_cores sg ix (Vptr bf Int.zero) args = Some c
+       , @find_symbol _ _ (my_cores ix).(Modsem.global) (my_cores ix).(Modsem.ge) id = Some v
+       , initCore my_cores sg ix v args = Some c
        & l' = pushCore l c pf]).
 Proof.
 rewrite/handle.
@@ -344,7 +346,7 @@ pattern (all (atExternal my_cores) (CallStack.callStack (stack l)))
  at 1 2 3 4 5 6 7 8 9.
 case f: (all _ _); move=> pf.
 case g: (fn_tbl l id)=> [ix|].
-case fnd: (Genv.find_symbol _ _)=> [bf|].
+case fnd: (find_symbol _ _)=> [bf|].
 case h: (initCore _ _ _)=> [c|].
 split=> H.
 exists (erefl true),ix,bf,c; split=> //; first by case: H=> <-.
@@ -363,9 +365,13 @@ Qed.
 
 End handle_lems.
 
-Definition main_sig := mksignature nil (Some Tint).
+Context (tysys : @TypeSys T V).
 
-Definition initial_core (ge: ge_ty) (v: val) (args: list val)
+(* Should this be an instance of something? *)
+Definition main_sig := {| g_sig_args := nil; g_sig_res := @main_typ _ _ tysys |}.
+
+(* Should this be an instance of something? *)
+(*Definition initial_core (ge: ge_ty) (v: val) (args: list val)
   : option (linker N my_cores) :=
   if v is Vptr bf ofs then 
   if Int.eq ofs Int.zero then
@@ -373,7 +379,14 @@ Definition initial_core (ge: ge_ty) (v: val) (args: list val)
   if my_fn_tbl id is Some ix then
   if initCore my_cores main_sig ix (Vptr bf Int.zero) args is Some c 
   then Some (mkLinker my_fn_tbl (CallStack.singl c))
-  else None else None else None else None else None.
+  else None else None else None else None else None.*)
+Definition initial_core (ge: G) (v: V) (args: list V)
+  : option (linker N my_cores) :=
+  if invert_symbol ge v is Some id then
+  if my_fn_tbl id is Some ix then
+  if initCore my_cores main_sig ix v args is Some c 
+  then Some (mkLinker my_fn_tbl (CallStack.singl c))
+  else None else None else None.
 
 (* Functions suffixed w/ 0 always operate on the running core on the (top *)
 (* of the) call stack.                                                    *)
@@ -382,29 +395,28 @@ Definition at_external0 (l: linker N my_cores) :=
   let: c   := peekCore l in
   let: ix  := c.(Core.i) in
   let: sem := (my_cores ix).(Modsem.sem) in
-  let: F   := (my_cores ix).(Modsem.F) in
-  let: V   := (my_cores ix).(Modsem.V) in
-    @at_external (Genv.t F V) _ _ sem (Core.c c).
+  let: G   := (my_cores ix).(Modsem.G) in
+    @at_external G _ _ _ _ sem (Core.c c).
 
 Arguments at_external0 !l.
 
-Require Import val_casted. (*for val_has_type_func*)
+(* Require Import val_casted. (*for val_has_type_func*)
+   TODO: Make a special instance for val. *)
 
 Definition halted0 (l: linker N my_cores) :=
   let: c   := peekCore l in
   let: ix  := c.(Core.i) in
   let: sg  := c.(Core.sg) in
   let: sem := (my_cores ix).(Modsem.sem) in
-  let: F   := (my_cores ix).(Modsem.F) in
-  let: V   := (my_cores ix).(Modsem.V) in
-    if @halted (Genv.t F V) _ _ sem (Core.c c) is Some v then
-      if val_casted.val_has_type_func v (proj_sig_res sg) then Some v
+  let: G   := (my_cores ix).(Modsem.G) in
+    if @halted G _ _ _ _ sem (Core.c c) is Some v then
+      if @has_type _ _ tysys v (g_sig_res sg) then Some v
       else None
     else None.
 
 Arguments halted0 !l.
 
-(* [corestep0] lifts a corestep of the runing core to a corestep of the   *)
+(* [corestep0] lifts a corestep of the running core to a corestep of the   *)
 (* whole program semantics.                                               *)
 
 Definition corestep0 
@@ -412,17 +424,16 @@ Definition corestep0
   let: c   := peekCore l in
   let: ix  := c.(Core.i) in
   let: sem := (my_cores ix).(Modsem.sem) in
-  let: F   := (my_cores ix).(Modsem.F) in
-  let: V   := (my_cores ix).(Modsem.V) in
+  let: G   := (my_cores ix).(Modsem.G) in
   let: ge  := (my_cores ix).(Modsem.ge) in
     exists c', 
-      @corestep (Genv.t F V) _ _ sem ge (Core.c c) m c' m'
+      @corestep G _ _ _ _ sem ge (Core.c c) m c' m'
    /\ l' = updCore l (Core.upd c c').
 
 Arguments corestep0 !l m l' m'.
 
-Definition fun_id (ef: external_function) : option ident :=
-  if ef is (EF_external id sig) then Some id else None.
+Definition fun_id {T : Type} (ef: g_external_function T) : option ident :=
+  if ef is (GEF_external id sig) then Some id else None.
 
 (* The linker is [at_external] whenever the top core is [at_external] and *)
 (* the [id] of the called external function isn't handleable by any       *)
@@ -435,14 +446,13 @@ Definition at_external (l: linker N my_cores) :=
          else Some (ef, dep_sig, args)
   else at_external0 l.
 
-Definition after_external (mv: option val) (l: linker N my_cores) :=
+Definition after_external (mv: option V) (l: linker N my_cores) :=
   let: c   := peekCore l in
   let: ix  := c.(Core.i) in
   let: sem := (my_cores ix).(Modsem.sem) in
-  let: F   := (my_cores ix).(Modsem.F) in
-  let: V   := (my_cores ix).(Modsem.V) in
+  let: G   := (my_cores ix).(Modsem.G) in
   let: ge  := (my_cores ix).(Modsem.ge) in
-    if @after_external (Genv.t F V) _ _ sem mv (Core.c c) 
+    if @after_external G _ _ _ _ sem mv (Core.c c) 
       is Some c' then Some (updCore l (Core.upd c c'))
     else None.
 
@@ -472,8 +482,8 @@ Definition corestep
          at_external) *)
 
       if at_external0 l is Some (ef, dep_sig, args) then
-      if fun_id ef is Some id then
-      if handle (ef_sig ef) id l args is Some l'' then l'=l'' else False else False
+      if ef is GEF_external id sig then
+      if handle sig id l args is Some l'' then l'=l'' else False else False
       else 
 
       (** 4- or halted, in which case we pop the halted core from the call stack
@@ -499,7 +509,7 @@ Inductive Corestep : linker N my_cores -> M
     Corestep l m (updCore l (Core.upd (peekCore l) c')) m'
 
 | Corestep_call :
-  forall (l : linker N my_cores) m ef dep_sig args id bf d_ix d
+  forall (l : linker N my_cores) m ef dep_sig args id sig v d_ix d
          (pf : all (atExternal my_cores) (CallStack.callStack l)),
 
   let: c := peekCore l in
@@ -508,15 +518,15 @@ Inductive Corestep : linker N my_cores -> M
   let: c_sem := Modsem.sem (my_cores c_ix) in
 
   semantics.at_external c_sem (Core.c c) = Some (ef,dep_sig,args) -> 
-  fun_id ef = Some id -> 
+  ef = GEF_external _ id sig -> 
   fn_tbl l id = Some d_ix -> 
-  Genv.find_symbol (my_cores d_ix).(Modsem.ge) id = Some bf -> 
+  @find_symbol _ _ (my_cores d_ix).(Modsem.global) (my_cores d_ix).(Modsem.ge) id = Some v -> 
 
   let: d_ge  := Modsem.ge (my_cores d_ix) in
   let: d_sem := Modsem.sem (my_cores d_ix) in
 
-  semantics.initial_core d_sem d_ge (Vptr bf Int.zero) args = Some d -> 
-  Corestep l m (pushCore l (Core.mk _ _ _ d (ef_sig ef)) pf) m
+  semantics.initial_core d_sem d_ge v args = Some d -> 
+  Corestep l m (pushCore l (Core.mk _ _ _ d sig) pf) m
 
 | Corestep_return : 
   forall (l : linker N my_cores) l'' m rv d',
@@ -537,7 +547,7 @@ Inductive Corestep : linker N my_cores -> M
   let: d_sem := Modsem.sem (my_cores d_ix) in
 
   semantics.halted c_sem (Core.c c) = Some rv -> 
-  val_has_type_func rv (proj_sig_res c_sg)=true -> 
+  @has_type _ _ tysys rv (g_sig_res c_sg)=true -> 
   semantics.after_external d_sem (Some rv) (Core.c d) = Some d' -> 
   Corestep l m (updCore l'' (Core.upd d d')) m.
 
@@ -552,12 +562,12 @@ split=> //.
 rewrite /corestep0=> [][]c' []step.
 by rewrite /= (corestep_not_at_external _ _ _ _ _ _ step) in A.
 rewrite /= in A.
-rewrite /inContext /at_external0 A H1.
+rewrite /inContext /at_external0 A.
 case e: (handle _ _ _)=> //[l'|].
-move: e; case/handleP=> pf' []ix' []bf' []c []C G D ->.
+move: e; case/handleP=> pf' []ix' []bf' []c []C G' D ->.
 move: D; rewrite /initCore.
 rewrite H2 in C; case: C=> eq; subst ix'.
-rewrite G in H3; case: H3=> ->.
+rewrite G' in H3; case: H3=> ->.
 by rewrite /= in H4; rewrite H4; case=> <-; f_equal; apply: proof_irr.
 move: e; rewrite/handle /pushCore.
 generalize (stack_push_wf l).
@@ -574,7 +584,7 @@ have at_ext:
   semantics.at_external
     (Modsem.sem (my_cores (Core.i (peekCore l))))
     (Core.c (peekCore l)) = None.
-{ case: (@at_external_halted_excl _ _ _
+{ case: (@at_external_halted_excl _ _ _ _ _
          (Modsem.sem (my_cores (Core.i (peekCore l))))
          (Core.c (peekCore l)))=> //.
   by rewrite /= in H2; rewrite H2. }
@@ -592,12 +602,13 @@ by apply: Corestep_step.
 case=> <-.
 case=> nstep.
 case atext: (at_external0 _)=> [[[ef dep_sig] args]|//].
-case funid: (fun_id ef)=> [id|//].
-case hdl:   (handle (ef_sig ef) id l args)=> [l''|//] ->.
+case funid: ef=> [id sig | // | // | // | // | // | // | // | // | // | // | //].
+(* There's probably a better way to do that, but I don't know ssreflect. -WM *)
+case hdl:   (handle sig id l args)=> [l''|//] ->.
 move: hdl; case/handleP=> pf []ix []bf []c []fntbl genv init ->.
 move: init; rewrite /initCore.
 case init: (semantics.initial_core _ _ _)=> [c'|//]; case=> <-. 
-by apply: (@Corestep_call _ _ ef dep_sig args id bf).
+by apply: (@Corestep_call _ _ ef dep_sig args id sig bf).
 case inCtx: (inContext _)=> //.
 case hlt: (halted0 _)=> [rv|//].
 case pop: (popCore _)=> [c|//].
@@ -606,7 +617,7 @@ move: aft; rewrite /after_external.
 case aft: (semantics.after_external _ _)=> [c''|//]. 
 rewrite /halted0 in hlt; move: hlt.
 case hlt: (semantics.halted _)=> //. 
-case oval: (val_has_type_func _ _)=> //; case=> Heq. subst. case=> <-.
+case oval: (has_type _ _)=> //; case=> Heq. subst. case=> <-.
 by apply: (@Corestep_return _ _ _ rv c'').
 Qed.
 
@@ -620,7 +631,7 @@ Proof. by move=>[]newCore []H1 H2; apply corestep_not_at_external in H1. Qed.
 
 Lemma at_external_halted_excl0 c : at_external0 c = None \/ halted0 c = None.
 Proof.
-case: (@at_external_halted_excl _ _ _
+case: (@at_external_halted_excl _ _ _ _ _
         (Modsem.sem (my_cores (Core.i (peekCore c))))
         (Core.c (peekCore c))).
 by rewrite /at_external0=> ->; left.
@@ -641,14 +652,14 @@ case Hht: (halted0 _)=>//.
 by move: Hht; rewrite/halted0; apply corestep_not_halted in H1; rewrite /= H1.
 Qed.
 
-Lemma corestep_not_at_external (ge : ge_ty) m c m' c' : 
+Lemma corestep_not_at_external (ge : G) m c m' c' : 
   corestep c m c' m' -> at_external c = None.
 Proof.
 rewrite/corestep/at_external.
 move=> [H|[_ [_ H]]]; first by move: H; move/corestep_not_at_external0=> /= ->.
 move: H; case Heq: (at_external0 c)=>[[[ef sig] args]|//].
 move: Heq; case: (at_external_halted_excl0 c)=> [H|H]; first by rewrite H.
-move=> H2; case: (fun_id ef)=>// id; case hdl: (handle _ _ _)=> [a|].
+move=> H2; case funid: ef=> [id sg | // | // | // | // | // | // | // | // | // | // | //]; case hdl: (handle _ _ _)=> [a|] /=.
 by move: hdl; case/handleP=> ? []? []? []? []->.
 by [].
 Qed.
@@ -662,7 +673,7 @@ move=> H; case Heq: (peekCore c)=>//[a].
 by case Hcx: (~~ inContext _)=>//; rewrite H.
 Qed.
 
-Lemma corestep_not_halted (ge : ge_ty) m c m' c' :
+Lemma corestep_not_halted (ge : G) m c m' c' :
   corestep c m c' m' -> halted c = None.
 Proof. 
 rewrite/corestep.
@@ -680,13 +691,13 @@ first by right; apply: (at_external0_not_halted _ Hat).
 by left.
 Qed.
 
-Definition coresem : CoreSemantics ge_ty (linker N my_cores) M :=
-  Build_CoreSemantics ge_ty (linker N my_cores) M 
+Definition coresem : CoreSemantics G (linker N my_cores) M V T :=
+  Build_CoreSemantics G (linker N my_cores) M V T
     initial_core
     at_external
     after_external
     halted 
-    (fun _ : ge_ty => corestep)
+    (fun _ : G => corestep)
     corestep_not_at_external    
     corestep_not_halted 
     at_external_halted_excl.
