core/extspec.v
@@ -4,22 +4,24 @@ Require Import Memory.
 
 Require Import ListSet.
 
+Require Import gen_genv.
+
 (** External function specifications and linking *)
 
-Structure external_specification (M E Z : Type) := 
+Structure external_specification (M V T E Z : Type) := 
   { ext_spec_type : E -> Type
   ; ext_spec_pre: forall e: E, 
-    ext_spec_type e -> list typ -> list val -> Z -> M -> Prop
+    ext_spec_type e -> list T -> list V -> Z -> M -> Prop
   ; ext_spec_post: forall e: E, 
-    ext_spec_type e -> option typ -> option val -> Z -> M ->  Prop
-  ; ext_spec_exit: option val -> Z -> M ->  Prop }.
+    ext_spec_type e -> option T -> option V -> Z -> M ->  Prop
+  ; ext_spec_exit: option V -> Z -> M ->  Prop }.
 
-Arguments ext_spec_type {M E Z} _ _.
-Arguments ext_spec_pre {M E Z} _ _ _ _ _ _ _.
-Arguments ext_spec_post {M E Z} _ _ _ _ _ _ _.
-Arguments ext_spec_exit {M E Z} _ _ _ _.
+Arguments ext_spec_type {M V T E Z} _ _.
+Arguments ext_spec_pre {M V T E Z} _ _ _ _ _ _ _.
+Arguments ext_spec_post {M V T E Z} _ _ _ _ _ _ _.
+Arguments ext_spec_exit {M V T E Z} _ _ _ _.
 
-Definition ext_spec := external_specification mem external_function.
+Definition ext_spec := external_specification mem val typ external_function.
 
 Lemma extfunct_eqdec (ef1 ef2 : external_function) : {ef1=ef2} + {~ef1=ef2}.
 Proof. 
@@ -29,11 +31,11 @@ Defined.
 
 Set Implicit Arguments.
 
-Definition ef_ext_spec (M Z : Type) := 
-  external_specification M AST.external_function Z.
+Definition ef_ext_spec (M V T Z : Type) := 
+  external_specification M V T (gen_genv.g_external_function T) Z.
 
 Definition spec_of 
-  (M Z : Type) (ef : AST.external_function) (spec : ef_ext_spec M Z) :=
+  (M V T Z : Type) (ef : g_external_function _) (spec : ef_ext_spec M V T Z) :=
   (ext_spec_pre spec ef, ext_spec_post spec ef).
 
 Definition oval_inject j (v tv : option val) :=
@@ -45,7 +47,7 @@ Definition oval_inject j (v tv : option val) :=
 
 Module ExtSpecProperties.
 
-Definition det (M E Z : Type) (spec : external_specification M E Z) :=
+Definition det (M V T E Z : Type) (spec : external_specification M V T E Z) :=
   forall ef (x x' : ext_spec_type spec ef) tys z vals m
          oty' ov' z' m' oty'' ov'' z'' m'',
   ext_spec_pre spec ef x tys vals z m -> 
