core/gen_genv.v
@@ -1,0 +1,122 @@
+(* A generalization of CompCert's global environments. *)
+Require Import Globalenvs.
+Require Import AST.
+Require Import Values.
+Require Import Integers.
+Require Import ZArith.
+Require Import Floats.
+
+Class GlobalEnv {G V : Type} := 
+  { find_symbol   : (* should we parameterize by ident as well? *) 
+                    G -> ident -> option V;
+    invert_symbol : G -> V -> option ident }.
+
+Instance GenvGlobal F V : @GlobalEnv (Genv.t F V) val :=
+  { find_symbol := fun ge i => option_map (fun bf => Vptr bf Int.zero) 
+                               (Genv.find_symbol ge i);
+    invert_symbol := fun ge v => match v with
+      | Vptr bf ofs => if Int.eq ofs Int.zero then Genv.invert_symbol ge bf
+                       else None
+      | _ => None
+      end }.
+
+Class TypeSys {T V : Type} :=
+  { has_type : V -> T -> bool; main_typ : T }.
+(* Can't make a CompCert instance of this here because it needs 
+   val_has_type_func from val_casted, which imports semantics. The specific
+   function doesn't actually depend on semantics, though, so this is fixable. *)
+
+
+Record g_signature (T : Type) : Type := {
+  g_sig_args: list T;
+  g_sig_res: T
+}.
+Arguments g_sig_args {T} _.
+Arguments g_sig_res {T} _.
+
+(* When should a typeclass be used, and when is a record better? *)
+Definition g_sig_of_sig (sg : signature) := 
+  {| g_sig_args := sig_args sg; g_sig_res := proj_sig_res sg |}.
+(* Does the result type need to be an option? None seems to be coerced
+   to int in the CompCert version. *)
+
+(* External functions with generalized signatures. 
+   These are still tied to CompCert memory_chunks for now. *)
+Inductive g_external_function (T : Type) : Type :=
+  | GEF_external (name: ident) (sg: g_signature T)
+     (** A system call or library function.  Produces an event
+         in the trace. *)
+  | GEF_builtin (name: ident) (sg: g_signature T)
+     (** A compiler built-in function.  Behaves like an external, but
+         can be inlined by the compiler. *)
+  | GEF_vload (chunk: memory_chunk)
+     (** A volatile read operation.  If the adress given as first argument
+         points within a volatile global variable, generate an
+         event and return the value found in this event.  Otherwise,
+         produce no event and behave like a regular memory load. *)
+  | GEF_vstore (chunk: memory_chunk)
+     (** A volatile store operation.   If the adress given as first argument
+         points within a volatile global variable, generate an event.
+         Otherwise, produce no event and behave like a regular memory store. *)
+  | GEF_vload_global (chunk: memory_chunk) (id: ident) (ofs: int)
+     (** A volatile load operation from a global variable. 
+         Specialized version of [EF_vload]. *)
+  | GEF_vstore_global (chunk: memory_chunk) (id: ident) (ofs: int)
+     (** A volatile store operation in a global variable. 
+         Specialized version of [EF_vstore]. *)
+  | GEF_malloc
+     (** Dynamic memory allocation.  Takes the requested size in bytes
+         as argument; returns a pointer to a fresh block of the given size.
+         Produces no observable event. *)
+  | GEF_free
+     (** Dynamic memory deallocation.  Takes a pointer to a block
+         allocated by an [EF_malloc] external call and frees the
+         corresponding block.
+         Produces no observable event. *)
+  | GEF_memcpy (sz: Z) (al: Z)
+     (** Block copy, of [sz] bytes, between addresses that are [al]-aligned. *)
+  | GEF_annot (text: ident) (targs: list (g_annot_arg T))
+     (** A programmer-supplied annotation.  Takes zero, one or several arguments,
+         produces an event carrying the text and the values of these arguments,
+         and returns no value. *)
+  | GEF_annot_val (text: ident) (targ: T)
+     (** Another form of annotation that takes one argument, produces
+         an event carrying the text and the value of this argument,
+         and returns the value of the argument. *)
+  | GEF_inline_asm (text: ident)
+     (** Inline [asm] statements.  Semantically, treated like an
+         annotation with no parameters ([EF_annot text nil]).  To be
+         used with caution, as it can invalidate the semantic
+         preservation theorem.  Generated only if [-finline-asm] is
+         given. *)
+
+with g_annot_arg (T : Type) : Type :=
+  | GAA_arg (ty: T)
+  | GAA_int (n: int)
+  | GAA_float (n: float).
+
+Definition gsig_to_sig (gsg : g_signature typ) : signature :=
+  {| sig_args := g_sig_args gsg; sig_res := Some (g_sig_res gsg) |}.
+
+Definition gaa_to_aa gaa :=
+  match gaa with 
+  | GAA_arg ty => AA_arg ty
+  | GAA_int n => AA_int n
+  | GAA_float n => AA_float n
+  end.
+
+Definition gef_to_ef (gef : g_external_function typ) : external_function :=
+  match gef with
+  | GEF_external name sg => EF_external name (gsig_to_sig sg)
+  | GEF_builtin name sg => EF_builtin name (gsig_to_sig sg)
+  | GEF_vload chunk => EF_vload chunk
+  | GEF_vstore chunk => EF_vstore chunk
+  | GEF_vload_global chunk id ofs => EF_vload_global chunk id ofs
+  | GEF_vstore_global chunk id ofs => EF_vstore_global chunk id ofs
+  | GEF_malloc => EF_malloc
+  | GEF_free => EF_free
+  | GEF_memcpy sz al => EF_memcpy sz al
+  | GEF_annot text targs => EF_annot text (List.map gaa_to_aa targs)
+  | GEF_annot_val text targ => EF_annot_val text targ
+  | GEF_inline_asm text => EF_inline_asm text
+  end.
